\documentclass{scrreprt} % comment this out when done editing
\usepackage{standalone}
\usepackage{chez}

% \NewDocumentCommand{\evalat}{sO{\big}mm}{%
%   \IfBooleanTF{#1}
%    {\mleft. #3 \mright|_{#4}}
%    {#3#2|_{#4}}%
% }

\begin{document}

\input{unit01/20210924.tex}

\subsection{August 24, 2021 - Derivatives}

\begin{example}[Parabolic]

Assume the graph is something generally parabolic, such as $f(t) = t^2$.

First, recall the second kinematic

$$
\Delta x = v_0t + \frac{1}{2}at^2
$$

Recall that for our tangent graphs (without the use of much calculs), we would
find the slope of a secant line. We would define the slope as

$$
v = \frac{\Delta x}{\Delta t}
$$

which would differ from the instantaneous velocity for the vast majority of the
time.

As a result, we take

$$
v = \lim_{\Delta x \rightarrow 0}\frac{x_f - x_i}{t_f - t_i}
$$

for

$$
\lim_{\Delta x \rightarrow 0}\frac{5(t + \Delta t)^2 - 5t^2}{t + \Delta t - t}
= \lim_{\Delta x \rightarrow 0}5\Delta t + 10t = 10t
$$

notice how this equation looks similar to $v = v_0 + at$ 

\end{example}

\begin{remark}[Historical Context - Leibniz and Newton]
	Derivative - coined by "Leibniz."
	
	Issues with naming it this way: derivative implies derivation, although the
	process itself of taking a derivative is differentation.

	$\Delta x$ was renamed from $\Delta x$ to $dx$. The only real velocity equation
	according to most univeristy professors is $$v = \frac{dy}{dx} = \frac{dx}{dt}$$

	Then, the acceleration equation becomes
	$$a = \frac{dv}{dt} = \frac{d}{dt}v = \frac{d^2y}{dx^2}$$
\end{remark}

\begin{remark}[Rules of Differentiation]
	A derivative is an expression that represents the rate of change of a function
	with respect to an independent variable.

	\begin{enumerate}
		\item Constant Rule. Example: if $x=6$, then $\frac{dy}{dx}=0$.
		\item Power rule: $$\frac{d}{dx}Cdt^n = (C \cdot n)t^{n-1}$$
	\end{enumerate}
\end{remark}

\begin{example}[Example]
	What is the squirrel's acceleration at $t=1$ second if its position is
	given by the equation $x = 2t^5 - 3t^2 + 2t - 4$?

	$$\frac{d}{dx} = 10t^4 - 6t + 2 = 40t^3 - 6$$
	$$\evalat{40t^3 - 6}{t = 1} = 34 m / s$$
\end{example}


\end{document}